dpe: copy context arrays instead of storing input arrays in global state. required pulse memcpy and refining seq types throughout DICE impl.

share/steel/examples/pulse/dice/l0/L0Core.fst
@@ -22,12 +22,13 @@ open Array
 
 ```pulse
 fn create_deviceIDCRI
-  (deviceID_pub: A.array U8.t)
-  (deviceIDCRI_len: U32.t)
-  (deviceIDCRI_buf: A.array U8.t)
+  (deviceID_pub: A.larray U8.t (US.v v32us))
+  (deviceIDCRI_len: US.t)
+  (deviceIDCRI_buf: A.larray U8.t (US.v deviceIDCRI_len))
   (deviceIDCSR_ingredients: deviceIDCSR_ingredients_t)
   (#pub_perm:perm)
-  (#pub#_buf:erased (Seq.seq U8.t))
+  (#pub:erased (elseq U8.t v32us)) 
+  (#_buf:erased (elseq U8.t deviceIDCRI_len))
   requires 
     A.pts_to deviceID_pub pub_perm pub **
     A.pts_to deviceIDCRI_buf full_perm _buf **
@@ -39,7 +40,7 @@ fn create_deviceIDCRI
                           deviceIDCSR_ingredients.s_country
     )
   ensures
-    exists (buf:Seq.seq U8.t).
+    exists (buf:elseq U8.t deviceIDCRI_len).
       A.pts_to deviceID_pub pub_perm pub **
       A.pts_to deviceIDCRI_buf full_perm buf **
       pure (
@@ -70,14 +71,16 @@ fn create_deviceIDCRI
 // TODO: don't need full perm on all of these
 ```pulse
 fn sign_and_finalize_deviceIDCSR
-  (deviceID_priv: A.array U8.t)
-  (deviceIDCRI_len: U32.t)
-  (deviceIDCRI_buf: A.array U8.t)
-  (deviceIDCSR_len: U32.t)
-  (deviceIDCSR_buf: A.array U8.t)
+  (deviceID_priv: A.larray U8.t (US.v v32us))
+  (deviceIDCRI_len: US.t)
+  (deviceIDCRI_buf: A.larray U8.t (US.v deviceIDCRI_len))
+  (deviceIDCSR_len: US.t)
+  (deviceIDCSR_buf: A.larray U8.t (US.v deviceIDCSR_len))
   (deviceIDCSR_ingredients: deviceIDCSR_ingredients_t)
   (#priv_perm:perm)
-  (#priv#_cri_buf#_csr_buf:erased (Seq.seq U8.t))
+  (#priv:erased (elseq U8.t v32us)) 
+  (#_cri_buf:erased (elseq U8.t deviceIDCRI_len)) 
+  (#_csr_buf:erased (elseq U8.t deviceIDCSR_len))
   requires (
     A.pts_to deviceID_priv priv_perm priv **
     A.pts_to deviceIDCRI_buf full_perm _cri_buf **
@@ -88,12 +91,12 @@ fn sign_and_finalize_deviceIDCSR
                           deviceIDCSR_ingredients.s_common
                           deviceIDCSR_ingredients.s_org
                           deviceIDCSR_ingredients.s_country /\
-      0 < U32.v deviceIDCRI_len /\ 
+      0 < US.v deviceIDCRI_len /\ 
       valid_deviceIDCSR_ingredients deviceIDCRI_len /\
       deviceIDCSR_len == length_of_deviceIDCSR deviceIDCRI_len
     ))
   ensures (
-    exists (csr_buf:Seq.seq U8.t). 
+    exists (csr_buf:elseq U8.t deviceIDCSR_len). 
     A.pts_to deviceID_priv priv_perm priv **
     A.pts_to deviceIDCRI_buf full_perm _cri_buf **
     A.pts_to deviceIDCSR_buf full_perm csr_buf **
@@ -110,16 +113,16 @@ fn sign_and_finalize_deviceIDCSR
               _cri_buf)))
     ))
 {
-  let deviceIDCRI_sig = new_array 0uy (u32_to_us deviceIDCRI_len);
+  let deviceIDCRI_sig = new_array 0uy deviceIDCRI_len;
 
-  ed25519_sign deviceIDCRI_sig deviceID_priv (u32_to_us deviceIDCRI_len) deviceIDCRI_buf;
+  ed25519_sign deviceIDCRI_sig deviceID_priv deviceIDCRI_len deviceIDCRI_buf;
 
   let deviceIDCSR = x509_get_deviceIDCSR
                       deviceIDCRI_len
                       deviceIDCRI_buf
                       deviceIDCRI_sig;
                     
-  serialize_deviceIDCSR deviceIDCRI_len deviceIDCSR deviceIDCSR_buf deviceIDCSR_len;
+  serialize_deviceIDCSR deviceIDCRI_len deviceIDCSR deviceIDCSR_len deviceIDCSR_buf;
 
   free_array deviceIDCRI_sig;
   ()
@@ -128,15 +131,17 @@ fn sign_and_finalize_deviceIDCSR
 
 ```pulse
 fn create_aliasKeyTBS
-  (fwid: A.larray U8.t 32)
+  (fwid: A.larray U8.t (US.v v32us))
   (authKeyID: A.array U8.t)
-  (deviceID_pub: A.larray U8.t 32)
-  (aliasKey_pub: A.larray U8.t 32)
-  (aliasKeyTBS_len: U32.t)
-  (aliasKeyTBS_buf: A.array U8.t)
+  (deviceID_pub: A.larray U8.t (US.v v32us))
+  (aliasKey_pub: A.larray U8.t (US.v v32us))
+  (aliasKeyTBS_len: US.t)
+  (aliasKeyTBS_buf: A.larray U8.t (US.v aliasKeyTBS_len))
   (aliasKeyCRT_ingredients: aliasKeyCRT_ingredients_t)
   (#fwid_perm #authKey_perm #device_perm #aliasKey_perm:perm)
-  (#fwid0 #authKeyID0 #deviceID_pub0 #aliasKey_pub0 #_buf:erased (Seq.seq U8.t))
+  (#fwid0 #authKeyID0: erased (Seq.seq U8.t))
+  (#deviceID_pub0 #aliasKey_pub0: erased (elseq U8.t v32us)) 
+  (#_buf:erased (elseq U8.t aliasKeyTBS_len))
   requires 
     A.pts_to fwid fwid_perm fwid0 **
     A.pts_to authKeyID authKey_perm authKeyID0 **
@@ -154,7 +159,7 @@ fn create_aliasKeyTBS
                           aliasKeyCRT_ingredients.s_country
                           aliasKeyCRT_ingredients.l0_version
     )
-  ensures exists (buf:Seq.seq U8.t).
+  ensures exists (buf:elseq U8.t aliasKeyTBS_len).
     A.pts_to fwid fwid_perm fwid0 **
     A.pts_to authKeyID authKey_perm authKeyID0 **
     A.pts_to deviceID_pub device_perm deviceID_pub0 **
@@ -185,14 +190,16 @@ fn create_aliasKeyTBS
 // TODO: don't need full perm on all of these
 ```pulse
 fn sign_and_finalize_aliasKeyCRT
-  (deviceID_priv: A.array U8.t)
-  (aliasKeyTBS_len: U32.t)
-  (aliasKeyTBS_buf: A.array U8.t)
-  (aliasKeyCRT_len: U32.t)
-  (aliasKeyCRT_buf: A.array U8.t)
+  (deviceID_priv: A.larray U8.t (US.v v32us))
+  (aliasKeyTBS_len: US.t)
+  (aliasKeyTBS_buf: A.larray U8.t (US.v aliasKeyTBS_len))
+  (aliasKeyCRT_len: US.t)
+  (aliasKeyCRT_buf: A.larray U8.t (US.v aliasKeyCRT_len))
   (aliasKeyCRT_ingredients: aliasKeyCRT_ingredients_t)
   (#priv_perm:perm)
-  (#priv#_tbs_buf#_crt_buf:erased (Seq.seq U8.t))
+  (#priv:erased (elseq U8.t v32us))
+  (#_tbs_buf:erased (elseq U8.t aliasKeyTBS_len))
+  (#_crt_buf:erased (elseq U8.t aliasKeyCRT_len))
   requires (
     A.pts_to deviceID_priv priv_perm priv **
     A.pts_to aliasKeyTBS_buf full_perm _tbs_buf **
@@ -207,12 +214,12 @@ fn sign_and_finalize_aliasKeyCRT
                           aliasKeyCRT_ingredients.s_org
                           aliasKeyCRT_ingredients.s_country
                           aliasKeyCRT_ingredients.l0_version /\
-      0 < U32.v aliasKeyTBS_len /\ 
+      0 < US.v aliasKeyTBS_len /\ 
       valid_aliasKeyCRT_ingredients aliasKeyTBS_len /\
       aliasKeyCRT_len == length_of_aliasKeyCRT aliasKeyTBS_len
     ))
   ensures (
-    exists (crt_buf:Seq.seq U8.t). 
+    exists (crt_buf:elseq U8.t aliasKeyCRT_len). 
     A.pts_to deviceID_priv priv_perm priv **
     A.pts_to aliasKeyTBS_buf full_perm _tbs_buf **
     A.pts_to aliasKeyCRT_buf full_perm crt_buf **
@@ -229,16 +236,16 @@ fn sign_and_finalize_aliasKeyCRT
               _tbs_buf)))
     ))
 {
-  let aliasKeyTBS_sig = new_array 0uy (u32_to_us aliasKeyTBS_len);
+  let aliasKeyTBS_sig = new_array 0uy aliasKeyTBS_len;
 
-  ed25519_sign aliasKeyTBS_sig deviceID_priv (u32_to_us aliasKeyTBS_len) aliasKeyTBS_buf;
+  ed25519_sign aliasKeyTBS_sig deviceID_priv aliasKeyTBS_len aliasKeyTBS_buf;
 
   let aliasKeyCRT = x509_get_aliasKeyCRT
                       aliasKeyTBS_len
                       aliasKeyTBS_buf
                       aliasKeyTBS_sig;
                     
-  serialize_aliasKeyCRT aliasKeyTBS_len aliasKeyCRT aliasKeyCRT_buf aliasKeyCRT_len;
+  serialize_aliasKeyCRT aliasKeyTBS_len aliasKeyCRT aliasKeyCRT_len aliasKeyCRT_buf;
 
   free_array aliasKeyTBS_sig;
   ()
@@ -249,22 +256,22 @@ fn sign_and_finalize_aliasKeyCRT
 
 let deviceIDCSR_pre 
   (deviceIDCSR: deviceIDCSR_ingredients_t) 
-  (deviceIDCRI_len: U32.t) 
-  (deviceIDCSR_len: U32.t) 
+  (deviceIDCRI_len: US.t) 
+  (deviceIDCSR_len: US.t) 
   : prop
   = deviceIDCRI_len == len_of_deviceIDCRI
                         deviceIDCSR.version
                         deviceIDCSR.s_common
                         deviceIDCSR.s_org
                         deviceIDCSR.s_country /\
-    0 < U32.v deviceIDCRI_len /\ 
+    0 < US.v deviceIDCRI_len /\ 
     valid_deviceIDCSR_ingredients deviceIDCRI_len /\
     deviceIDCSR_len == length_of_deviceIDCSR deviceIDCRI_len
 
 let aliasKeyCRT_pre 
   (aliasKeyCRT:aliasKeyCRT_ingredients_t) 
-  (aliasKeyTBS_len:U32.t) 
-  (aliasKeyCRT_len:U32.t) 
+  (aliasKeyTBS_len:US.t) 
+  (aliasKeyCRT_len:US.t) 
   : prop
   = aliasKeyTBS_len == len_of_aliasKeyTBS
                         aliasKeyCRT.serialNumber
@@ -275,7 +282,7 @@ let aliasKeyCRT_pre
                         aliasKeyCRT.s_org
                         aliasKeyCRT.s_country
                         aliasKeyCRT.l0_version /\
-    0 < U32.v aliasKeyTBS_len /\ 
+    0 < US.v aliasKeyTBS_len /\ 
     valid_aliasKeyCRT_ingredients aliasKeyTBS_len /\
     aliasKeyCRT_len == length_of_aliasKeyCRT aliasKeyTBS_len
 
@@ -286,8 +293,8 @@ let aliasKey_post
   (fwid:Seq.seq U8.t)
   (aliasKey_label_len:hkdf_lbl_len)
   (aliasKey_label:Seq.seq U8.t)
-  (aliasKey_pub:Seq.seq U8.t)
-  (aliasKey_priv:Seq.seq U8.t)
+  (aliasKey_pub:elseq U8.t v32us)
+  (aliasKey_priv:elseq U8.t v32us)
   : prop
   = (aliasKey_pub, aliasKey_priv) == derive_AliasKey_spec alg dig_len cdi fwid aliasKey_label_len aliasKey_label
 
@@ -298,8 +305,8 @@ let deviceIDCSR_post
   (deviceID_label_len: hkdf_lbl_len)
   (deviceID_label: Seq.seq U8.t)
   (deviceIDCSR_ingredients: deviceIDCSR_ingredients_t)
-  (deviceIDCSR_len: U32.t)
-  (deviceIDCSR_buf: Seq.seq U8.t)
+  (deviceIDCSR_len: US.t)
+  (deviceIDCSR_buf: elseq U8.t deviceIDCSR_len)
   : prop
   = let (deviceID_pub, deviceID_priv) = (derive_DeviceID_spec alg dig_len cdi deviceID_label_len deviceID_label) in 
     let deviceIDCRI_len = len_of_deviceIDCRI 
@@ -335,9 +342,9 @@ let aliasKeyCRT_post
   (deviceID_label_len:hkdf_lbl_len)
   (deviceID_label:Seq.seq U8.t)
   (aliasKeyCRT_ingredients:aliasKeyCRT_ingredients_t)
-  (aliasKeyCRT_len:U32.t)
-  (aliasKeyCRT_buf:Seq.seq U8.t)
-  (aliasKey_pub:Seq.seq U8.t)
+  (aliasKeyCRT_len:US.t)
+  (aliasKeyCRT_buf:elseq U8.t aliasKeyCRT_len)
+  (aliasKey_pub:elseq U8.t v32us)
   : prop
   = let (deviceID_pub, deviceID_priv) = (derive_DeviceID_spec alg dig_len cdi deviceID_label_len deviceID_label) in 
     let authKeyID = derive_AuthKeyID_spec alg deviceID_pub in
@@ -371,18 +378,20 @@ let aliasKeyCRT_post
 ```pulse
 fn l0_main
   (cdi: A.larray U8.t (US.v dice_digest_len))
-  (aliasKey_pub: A.larray U8.t 32)
-  (aliasKey_priv: A.larray U8.t 32)
-  (aliasKeyTBS_len:U32.t)
-  (aliasKeyCRT_len:U32.t)
-  (aliasKeyCRT: A.array U8.t)
-  (deviceIDCRI_len:U32.t)
-  (deviceIDCSR_len:U32.t)
-  (deviceIDCSR: A.array U8.t)
+  (aliasKey_pub: A.larray U8.t (US.v v32us))
+  (aliasKey_priv: A.larray U8.t (US.v v32us))
+  (aliasKeyTBS_len:US.t)
+  (aliasKeyCRT_len:US.t)
+  (aliasKeyCRT: A.larray U8.t (US.v aliasKeyCRT_len))
+  (deviceIDCRI_len:US.t)
+  (deviceIDCSR_len:US.t)
+  (deviceIDCSR: A.larray U8.t (US.v deviceIDCSR_len))
   (record: l0_record_t)
-  (#repr: Ghost.erased l0_record_repr)
-  (#cdi0:Ghost.erased (elseq U8.t dice_digest_len))
-  (#aliasKey_pub0 #aliasKey_priv0 #aliasKeyCRT0 #deviceIDCSR0: Ghost.erased (Seq.seq U8.t))
+  (#repr: erased l0_record_repr)
+  (#cdi0:erased (elseq U8.t dice_digest_len))
+  (#aliasKey_pub0 #aliasKey_priv0:erased (elseq U8.t v32us)) 
+  (#aliasKeyCRT0: elseq U8.t aliasKeyCRT_len)
+  (#deviceIDCSR0: elseq U8.t deviceIDCSR_len)
   requires (
     l0_record_perm record repr **
     A.pts_to cdi full_perm cdi0 **
@@ -398,7 +407,9 @@ fn l0_main
   ensures (
       l0_record_perm record repr **
       A.pts_to cdi full_perm (Seq.create (US.v dice_digest_len) 0uy) **
-      exists (aliasKey_pub1 aliasKey_priv1 aliasKeyCRT1 deviceIDCSR1:Seq.seq U8.t). (
+      exists (aliasKey_pub1 aliasKey_priv1:elseq U8.t v32us) 
+             (aliasKeyCRT1:elseq U8.t aliasKeyCRT_len)
+             (deviceIDCSR1:elseq U8.t deviceIDCSR_len). (
         A.pts_to aliasKey_pub full_perm aliasKey_pub1 **
         A.pts_to aliasKey_priv full_perm aliasKey_priv1 **
         A.pts_to aliasKeyCRT full_perm aliasKeyCRT1 **
@@ -421,8 +432,8 @@ fn l0_main
 {
   unfold l0_record_perm record repr;
 
-  let deviceID_pub = new_array 0uy 32sz;
-  let deviceID_priv = new_array 0uy 32sz;
+  let deviceID_pub = new_array 0uy v32us;
+  let deviceID_priv = new_array 0uy v32us;
   derive_DeviceID dice_hash_alg 
     deviceID_pub deviceID_priv cdi 
     record.deviceID_label_len record.deviceID_label
@@ -436,7 +447,7 @@ fn l0_main
   derive_AuthKeyID dice_hash_alg
     authKeyID deviceID_pub;
 
-  let deviceIDCRI = new_array 0uy (u32_to_us deviceIDCRI_len);
+  let deviceIDCRI = new_array 0uy deviceIDCRI_len;
   create_deviceIDCRI deviceID_pub
     deviceIDCRI_len deviceIDCRI
     record.deviceIDCSR_ingredients;
@@ -446,7 +457,7 @@ fn l0_main
     deviceIDCSR_len deviceIDCSR
     record.deviceIDCSR_ingredients;
 
-  let aliasKeyTBS = new_array 0uy (u32_to_us aliasKeyTBS_len);
+  let aliasKeyTBS = new_array 0uy aliasKeyTBS_len;
   create_aliasKeyTBS record.fwid authKeyID
     deviceID_pub aliasKey_pub
     aliasKeyTBS_len aliasKeyTBS
@@ -457,11 +468,15 @@ fn l0_main
     aliasKeyCRT_len aliasKeyCRT
     record.aliasKeyCRT_ingredients;
   
-  free_array deviceID_pub;
-  free_array deviceID_priv;
+  with s1. assert (A.pts_to deviceID_pub full_perm s1);
+  with s2. assert (A.pts_to deviceID_priv full_perm s2);
+  with s3. assert (A.pts_to deviceIDCRI full_perm s3);
+  with s4. assert (A.pts_to aliasKeyTBS full_perm s4);
+  free_array deviceID_pub #(coerce v32us s1);
+  free_array deviceID_priv #(coerce v32us s2);
   free_array authKeyID;
-  free_array deviceIDCRI;
-  free_array aliasKeyTBS;
+  free_array deviceIDCRI #(coerce deviceIDCRI_len s3);
+  free_array aliasKeyTBS #(coerce aliasKeyTBS_len s4);
 
   fold l0_record_perm record repr;
 
